code/ecdsa/Hacl.Impl.EC.PointDouble.fsti
@@ -14,8 +14,7 @@ open Spec.ECC.Curves
 
 open Hacl.Spec.MontgomeryMultiplication
 
-
-[@CInline]
+inline_for_extraction noextract
 val point_double: #c: curve -> p: point c -> result: point c 
   -> tempBuffer: lbuffer uint64  (getCoordinateLenU64 c *! 17ul) 
   -> Stack unit
